\documentclass{ximera}

\title{Practice for More Fourier}

\input{../../preamble}

\begin{document}
\begin{abstract}
Why?
\end{abstract}
\maketitle


\begin{exercise}
    Let
    \begin{equation*}
        f(t) =
        \begin{cases}
            0 & \text{if } \; {-1} < t \leq 0 , \\
            t & \text{if } \; \phantom{-}0 < t \leq  1 ,
        \end{cases}
    \end{equation*}
    extended periodically.
    \begin{itemize}
        \item Compute the Fourier series for $f(t)$.
        \item Write out the series explicitly up to the $3^{\text{rd}}$ harmonic.
    \end{itemize}
\end{exercise}

\begin{exercise}\%
    Let
    \begin{equation*}
        f(t) = t^2 \qquad \text{for } \; {-2} < t \leq 2
    \end{equation*}
    extended periodically.
    \begin{itemize}
        \item Compute the Fourier series for $f(t)$.
        \item Write out the series explicitly up to the $3^{\text{rd}}$ harmonic.
    \end{itemize}
\end{exercise}
%\exsol{%
%a) $\frac{8}{6} +
%\sum\limits_{n=1}^\infty
%\frac{16{(-1)}^n}{\pi^2 n^2}
%\cos\bigl(\frac{n\pi}{2} t\bigr)$
%\quad
%b) $\frac{8}{6}
%-
%\frac{16}{\pi^2 }
%\cos\bigl(\frac{\pi}{2} t\bigr)
%+
%\frac{4}{\pi^2}
%\cos\bigl(\pi t\bigr)
%-
%\frac{16}{9\pi^2}
%\cos\bigl(\frac{3\pi}{2} t\bigr) + \cdots$
%}

\begin{exercise}
    Let
    \begin{equation*}
        f(t) =
        \begin{cases}
            -t & \text{if } \; {-1} < t \leq 0 , \\
            t^2 & \text{if } \; \phantom{-}0 < t \leq  1 ,
        \end{cases}
    \end{equation*}
    extended periodically.
    \begin{itemize}
        \item Compute the Fourier series for $f(t)$.
        \item Write out the series explicitly up to the $3^{\text{rd}}$ harmonic.
    \end{itemize}
\end{exercise}

\begin{exercise}\%
    Let
    \begin{equation*}
        f(t) = t \qquad \text{for } \; {-\lambda} < t \leq \lambda \; \text{ (for some } \lambda > 0 \text{)}
    \end{equation*}
    extended periodically.
    \begin{itemize}
        \item Compute the Fourier series for $f(t)$.
        \item Write out the series explicitly up to the $3^{\text{rd}}$ harmonic.
    \end{itemize}
\end{exercise}
%\exsol{%
%a)
%$\sum\limits_{n=1}^\infty
%\frac{{(-1)}^{n+1}2\lambda}{n \pi}
%\sin\bigl(\frac{n\pi}{\lambda} t\bigr)$
%\quad
%b)
%$\frac{2\lambda}{\pi}
%\sin\bigl(\frac{\pi}{\lambda} t\bigr)
%-
%\frac{\lambda}{\pi}
%\sin\bigl(\frac{2\pi}{\lambda} t\bigr)
%+
%\frac{2\lambda}{3\pi}
%\sin\bigl(\frac{3\pi}{\lambda} t\bigr) - \cdots$
%}

\begin{exercise}
    Let
    \begin{equation*}
        f(t) =
        \begin{cases}
            \frac{-t}{10} & \text{if } \; {-10} < t \leq 0 , \\
            \frac{t}{10} & \text{if } \; \phantom{-1}0 < t \leq  10 ,
        \end{cases}
    \end{equation*}
    extended periodically (period is 20).
    \begin{itemize}
        \item Compute the Fourier series for $f(t)$.
        \item Write out the series explicitly up to the $3^{\text{rd}}$ harmonic.
    \end{itemize}
\end{exercise}

\begin{exercise}\%
    Let
    \begin{equation*}
        f(t) = \frac{1}{2} + \sum_{n=1}^\infty \frac{1}{n(n^2+1)} \sin(n\pi t) .
    \end{equation*}
    Compute $f'(t)$.
\end{exercise}
%\exsol{%
%$f'(t) = \sum\limits_{n=1}^\infty
%\frac{\pi}{n^2+1}
%\cos(n\pi t)$
%}

\begin{exercise}
    Let $f(t) = \sum_{n=1}^\infty \frac{1}{n^3} \cos (n t)$.  Is $f(t)$ continuous and differentiable everywhere?  Find the derivative (if it exists everywhere) or justify why $f(t)$ is not differentiable everywhere.
\end{exercise}

\begin{exercise}
    Let $f(t) = \sum_{n=1}^\infty \frac{{(-1)}^n}{n} \sin (n t)$.  Is $f(t)$ differentiable everywhere?  Find the derivative (if it exists everywhere) or justify why $f(t)$ is not differentiable everywhere.
\end{exercise}

\begin{exercise}\%
    Let
    \begin{equation*}
        f(t) = \frac{1}{2} + \sum_{n=1}^\infty \frac{1}{n^3} \cos(n t) .
    \end{equation*}
    \begin{itemize}
        \item Find the antiderivative.
        \item Is the antiderivative periodic?
    \end{itemize}
\end{exercise}
%\exsol{%
%a)
%$F(t) = \frac{t}{2} + C + \sum\limits_{n=1}^\infty
%\frac{1}{n^4}
%\sin(nt)$
%\qquad
%b) no
%}

\begin{exercise}
    Let
    \begin{equation*}
        f(t) =
        \begin{cases}
            0 & \text{if } \; {-2} < t \leq 0, \\
            t & \text{if } \; \phantom{-}0 < t \leq 1, \\
            -t+2 & \text{if } \; \phantom{-}1 < t \leq 2,
        \end{cases}
    \end{equation*}
    extended periodically.
    \begin{itemize}
        \item Compute the Fourier series for $f(t)$.
        \item Write out the series explicitly up to the $3^{\text{rd}}$ harmonic.
    \end{itemize}
\end{exercise}

\begin{exercise}
    Let
    \begin{equation*}
        f(t) = e^t \qquad \text{for } \; {-1} < t \leq 1
    \end{equation*}
    extended periodically.
    \begin{itemize}
        \item Compute the Fourier series for $f(t)$.
        \item Write out the series explicitly up to the $3^{\text{rd}}$ harmonic.
        \item What does the series converge to at $t=1$.
    \end{itemize}
\end{exercise}

\begin{exercise}
    Let
    \begin{equation*}
        f(t) = t^2 \qquad \text{for } \; {-1} < t \leq 1
    \end{equation*}
    extended periodically.
    \begin{itemize}
        \item Compute the Fourier series for $f(t)$.
        \item By plugging in $t=0$, evaluate $\displaystyle \sum_{n=1}^\infty \frac{{(-1)}^n}{n^2} = 1 - \frac{1}{4} + \frac{1}{9} - \cdots$.
        \item Now evaluate $\displaystyle \sum_{n=1}^\infty \frac{1}{n^2} = 1 + \frac{1}{4} + \frac{1}{9} + \cdots$.
    \end{itemize}
\end{exercise}

\begin{exercise}\%
    Let
    \begin{equation*}
        f(t) = \frac{t}{2} \qquad \text{for } \; {-\pi} < t < \pi
    \end{equation*}
    extended periodically.
    \begin{itemize}
        \item Compute the Fourier series for $f(t)$.
        \item Plug in $t=\frac{\pi}{2}$ to find a series representation for $\frac{\pi}{4}$.
        \item Using the first 4 terms of the result from part b) approximate $\frac{\pi}{4}$.
    \end{itemize}
\end{exercise}
%\exsol{%
%a)
%$\sum\limits_{n=1}^\infty
%\frac{{(-1)}^{n+1}}{n} \sin(nt)$
%\qquad
%b) $f$ is continuous at $t=\frac{\pi}{2}$ so the
%Fourier series converges to $f(\frac{\pi}{2}) = \frac{\pi}{4}$.
%Obtain
%$\frac{\pi}{4} = \sum\limits_{n=1}^\infty
%\frac{{(-1)}^{n+1}}{2n-1} = 1 - \frac{1}{3} + \frac{1}{5}-
%\frac{1}{7} + \cdots$.
%\qquad
%c) Using the first 4 terms get $\frac{76}{105}\approx 0.72$ (quite a bad
%approximation, you would have to take about 50 terms to start to get to
%within $0.01$ of $\frac{\pi}{4}$).
%}

\begin{exercise}
    Let
    \begin{equation*}
        f(t) =
        \begin{cases}
            0 & \text{if } \; {-3} < t \leq 0, \\
            t & \text{if } \; \phantom{-}0 < t \leq 3,
        \end{cases}
    \end{equation*}
    extended periodically.  Suppose $F(t)$ is the function given by the Fourier series of $f$.  Without computing the Fourier series evaluate
    \begin{itemize}
        \item $F(2)$
        \item $F(-2)$
        \item $F(4)$
        \item $F(-4)$
        \item $F(3)$
        \item $F(-9)$
    \end{itemize}
\end{exercise}

\begin{exercise}\%
    Let
    \begin{equation*}
        f(t) = 
        \begin{cases}
            0 & \text{if } \; {-2} < t \leq 0, \\
            2 & \text{if } \; \phantom{-}0 < t \leq 2,
        \end{cases}
    \end{equation*}
    extended periodically.  Suppose $F(t)$ is the function given by the Fourier series of $f$.  Without computing the Fourier series evaluate
    \begin{itemize}
        \item $F(0)$
        \item $F(-1)$
        \item $F(1)$
        \item $F(-2)$
        \item $F(4)$
        \item $F(-8)$
    \end{itemize}
\end{exercise}
%\exsol{%
%a) $F(0) = 1$, 
%b) $F(-1) = 0$, 
%c) $F(1) = 2$, 
%d) $F(-2) = 1$, 
%e) $F(4) = 1$, 
%f) $F(-9) = 0$ 
%}

%\setcounter{exercise}{100}


\end{document}