\documentclass{ximera}

\title{Practice for Solving Exact ODEs}

\input{../../preamble}

\begin{document}
\begin{abstract}
    Why?
\end{abstract}
\maketitle

\begin{exercise}
    Solve the following exact equations, implicit general solutions will suffice:
    \begin{itemize}
        \item $(2 xy + x^2) dx + (x^2+y^2+1) dy = 0$, $\answer{x^2y + \frac{x^3}{3} + \frac{y^3}{3} + y} = C$
        \item $x^5 + y^5 \frac{dy}{dx} = 0$, $\answer{\frac{x^6}{6} + \frac{y^6}{6}} = C$
        \item $e^x+y^3 + 3xy^2 \frac{dy}{dx} = 0$, $\answer{e^x + xy^3} = C$
        \item $(x+y)\cos(x)+\sin(x) + \sin(x)y' = 0$, $\answer{(x+y)\sin(x) + \cos(x)} = C$
    \end{itemize}
\end{exercise}
%\comboSol{%
%}
%{%
%a)~ $x^2y + \frac{x^3}{3} + \frac{y^3}{3} + y = C$ \quad b)~ $\frac{x^6}{6} + \frac{y^6}{6} = C$ \quad
%c)~ $e^x + xy^3 = C$ \quad d)~ $(x+y)\sin(x) + \cos(x) = C$
%}

\begin{exercise}%
    Solve the following exact equations, implicit general solutions will suffice:
    \begin{itemize}
        \item $\cos(x)+ye^{xy} + xe^{xy} y' = 0$, $\answer{e^{xy}+\sin(x)} = C$
        \item $(2x+y)dx + (x-4y) dy = 0$, $\answer{x^2+xy-2y^2} = C$
        \item $e^x + e^y \frac{dy}{dx} = 0$, $\answer{e^x+e^y} = C$
        \item $(3x^2+3y)dx + (3y^2+3x)dy = 0$, $\answer{x^3 + 3xy+ y^3} = C$
    \end{itemize}
\end{exercise}
%\exsol{%
%a) $e^{xy}+\sin(x)=C$ \quad
%b) $x^2+xy-2y^2=C$ \quad
%c) $e^x+e^y=C$ \quad
%d) $x^3 + 3xy+ y^3 = C$
%}

\begin{exercise}
    Solve the differential equation $(2ye^{2xy} - 2x) + (2xe^{2xy} + \cos(y))y' = 0$
    \[
        C = \answer{e^{2xy} - x^2 + \sin(y)}
    \]
\end{exercise}
%\comboSol{%
%}
%{%
%$e^{2xy} - x^2 + \sin(y) = C$
%}

\begin{exercise}
    Solve the differential equation $(-y\sin(xy) - 2xe^{x^2}) + (-x\sin(xy) + 1)y' = 0$
    \[
        C = \answer{\cos(xy) - e^{x^2} + y}
    \]
\end{exercise}
%\comboSol{%
%}
%{%
%$\cos(xy) - e^{x^2} + y = C$
%}

\begin{exercise}
    
    Solve the differential equation $(2x + 3y\sin(xy)) + (3x\sin(xy) - e^y)y' = 0$ with $y(2) = 0$.
    
    [Note: Make sure to enter the full equation, e.g. 0 = x + 4]
    \[
        \answer{x^2 - 3\cos(xy) - e^y = 0}
    \]
    
\end{exercise}
%\comboSol{%
%}
%{%
%$x^2 - 3\cos(xy) - e^y = 0$
%}

\begin{exercise}
    Solve the differential equation $x + yy' = 0$ with $y(0) = 8$. Write this as an explicit function.
    [Note: Make sure to enter the full equation, e.g. 0 = x + 4]
    \[
        \answer{y = \sqrt{64-x^2}}
    \]
    \begin{problem}
        Determine the interval of $x$ values where the solution is valid:
        \wordChoice{\choice{(}\choice[correct]{[}}$\answer{-8},\answer{8}$\wordChoice{\choice{)}\choice[correct]{]}}
    \end{problem}
    
\end{exercise}
%\comboSol{%
%}
%{%
%$y = \sqrt{64-x^2}$, valid on $[-8, 8]$
%}

\begin{exercise}
    Solve the differential equation $2x-2 + (8y+16)y' = 0$ with $y(2) = 0$. Write this as an explicit function.
    [Note: Make sure to enter the full equation, e.g. 0 = x + 4]
    \[
        \answer{y = \frac{-4 + \sqrt{17 - (x-1)^2}}{2}}
    \]
    \begin{problem}
        Determine the interval of $x$ values where the solution is valid:
        \wordChoice{\choice{(}\choice[correct]{[}}$\answer{1 - \sqrt{17}},\answer{1 + \sqrt{17}}$\wordChoice{\choice{)}\choice[correct]{]}}
    \end{problem}
\end{exercise}
%\comboSol{%
%}
%{%
%$y = \frac{-4 + \sqrt{17 - (x-1)^2}}{2}$, valid on $[1 - \sqrt{17}, 1 +\sqrt{17}]$
%}

\begin{exercise}
    Find the integrating factor for the following equations making them into exact equations. You can either use the formulas in this section or guess what the integrating factor should be.
    \begin{itemize}
        \item $e^{xy} dx + \frac{y}{x} e^{xy} dy = 0$, $\answer{xe^{-xy}}$
        \item $\frac{e^x+y^3}{y^2} dx + 3x dy = 0$, $\answer{y^2}$
        \item $(4x^5 + 9x^4y^2 + 10\frac{y}{x})dx + (6x^5y + 3x^2y^2 - 5)dy = 0$, $\answer{x^{-2}}$
        \item $2\sin(y) dx + x\cos(y)dy = 0$, $\answer{x}$
    \end{itemize}
\end{exercise}
%\comboSol{%
%}
%{%
%a)~ $xe^{-xy}$ \quad b)~$y^2$ \quad c)~$x^{-2}$ \quad d)~$x$
%}


\begin{exercise}%
    Find the integrating factor for the following equations making them into exact equations:
    \begin{itemize}
        \item $\frac{1}{y}dx + 3y dy = 0$, 
            Integrating Factor: $\answer{y}$,
            Exact Equation: $\answer{dx + 3y^2dy = 0}$
        \item $dx - e^{-x-y} dy = 0$, $\answer{xe^{-xy}}$, 
            Integrating Factor: $\answer{e^x}$,
            Exact Equation: $\answer{e^x dx - e^{-y}dy= 0}$
        \item $\bigl( \frac{\cos(x)}{y^2} + \frac{1}{y} \bigr) dx + \frac{x}{y^2} dy = 0$, $\answer{xe^{-xy}}$, 
            Integrating Factor: $\answer{y^2}$,
            Exact Equation: $\answer{(\cos(x)+y)dx + xdy = 0}$
        \item $\bigl( 2y + \frac{y^2}{x} \bigr) dx + ( 2y+x )dy = 0$, $\answer{xe^{-xy}}$, 
            Integrating Factor: $\answer{x}$,
            Exact Equation: $\answer{( 2xy+y^2 )dx + (x^2+2xy)dy = 0}$
    \end{itemize}
\end{exercise}

%\exsol{%
%a) Integrating factor is $y$, equation becomes $dx + 3y^2dy = 0$.
%\quad
%b) Integrating factor is $e^x$, equation becomes $e^x dx - e^{-y}dy
%= 0$.
%\quad
%c) Integrating factor is $y^2$, equation becomes $(\cos(x)+y)dx +
%xdy = 0$.
%\quad
%d) Integrating factor is $x$, equation becomes $( 2xy+y^2 )dx +
%(x^2+2xy)dy = 0$.
%}

\begin{exercise}
    Suppose you have an equation of the form: $f(x) + g(y) \frac{dy}{dx} = 0$.
    
    Is it exact? \wordChoice{\choice[correct]{Yes.}\choice{No.}}
    \begin{problem}
        Find the form of the potential function in terms of $f$ and $g$. 
        \[
            \int \answer{f(x)}dx + \int \answer{g(y)}dy = 0.
        \]
    \end{problem}
\end{exercise}
%\comboSol{%
%}
%{%
%a)~Yes. \quad b)~ $\int f(x)\ dx + \int g(y)\ dy = C$
%}

\begin{exercise}
    Suppose that we have the equation $f(x) dx - dy = 0$.
    
    Is this equation exact? \wordChoice{\choice[correct]{Yes.}\choice{No.}}
    \begin{problem}
        Find the general solution using a definite integral. $y = \int \answer{f(x)}dx + C$
    \end{problem}
\end{exercise}
%\comboSol{%
%}
%{%
%a)~ Yes. \quad b)~$y = \int f(x)\ dx + C$ 
%}

\begin{exercise}
    Find the potential function $F(x,y)$ of the exact equation $\frac{1+xy}{x}dx + \bigl(\frac{1}{y} + x \bigr) dy = 0$ in two different ways.
    \begin{itemize}
        \item Integrate $M$ in terms of $x$ and then differentiate in $y$ and set to $N$. $\answer{xy + \ln(x) + \ln(y) = C}$
        \item Integrate $N$ in terms of $y$ and then differentiate in $x$ and set to $M$. $\answer{xy + \ln(x) + \ln(y) = C}$
    \end{itemize}
\end{exercise}
%\comboSol{%
%}
%{%
%$xy + \ln(x) + \ln(y) = C$
%}

\begin{exercise}
    A function $u(x,y)$ is said to be a \emph{harmonic function} if $u_{xx} + u_{yy} = 0$.
    
    Compute: the difference between $M_y = -u_{yy}$ and $N_x = u_{xx}$: $\answer{0}$.
    \begin{problem}
        Since the difference is zero, they are equal, thus $-u_y dx + u_x dy = 0$ is an exact equation.  So there exists (at least locally) the so-called \emph{harmonic conjugate} function $v(x,y)$ such that $v_x = -u_y$ and $v_y = u_x$.
        
        Verify that the following $u$ are harmonic and find the corresponding harmonic conjugates $v$:
        \begin{itemize}
            \item $u = 2xy$, corresponding harmonic conjugate: $\answer{y^2 - x^2}$.
            \item $u = e^x \cos y$, corresponding harmonic conjugate: $\answer{e^{x}\sin(y)}$.
            \item $u = x^3-3xy^2$, corresponding harmonic conjugate: $\answer{3x^2y - y^3}$.
        \end{itemize}
    \end{problem}
\end{exercise}
%\comboSol{%
%}
%{%
%a)~ $M_y = -u_{yy}$ and $N_x = u_{xx}$, and the difference is zero, so they are equal. \\
%b)~ (i)~$y^2 - x^2$ \quad (ii)~$e^{x}\sin(y)$ \quad (iii)~ $3x^2y - y^3$
%}

\begin{exercise}\label{ex:separableExact}%
    Consider equations of the form $y' = f(x)g(y)$. Compute: $M_y = \answer{0}$, and $N_x = \answer{0}$.
    \begin{problem}
        Since $M_y = 0 = N_x$, we know that it is an exact function. We can thus use the substitution $y' = xy$ to rewrite it as an exact equation and solve. Start by using separation of variables to get:
        \[
            \answer{-x }dx + \answer{\frac{1}{y}} dy = 0
        \]
        \begin{problem}
            Then taking the integral we get:
            \[
                F(x,y) = \answer{-\frac{x^2}{2} + \ln \lvert y \rvert} + C
            \]
        \end{problem}
    \end{problem}
\end{exercise}
%\exsol{%
%a) The equation is $ - f(x) dx + \frac{1}{g(y)} dy$,
%and this is exact
%because $M = -f(x)$, $N = \frac{1}{g(y)}$, so $M_y = 0 = N_x$.
%\quad
%b) $-x dx + \frac{1}{y} dy = 0$, leads to
%potential function $F(x,y) = -\frac{x^2}{2} + \ln \lvert y \rvert$, solving
%$F(x,y) = C$ leads to the same solution as the example.
%}

%\setcounter{exercise}{100}



\end{document}