\documentclass{ximera}

\title{Practice for Solving First Order Linear ODEs}

\input{../../preamble}

\begin{document}
\begin{abstract}
    Why?
\end{abstract}
\maketitle


In the exercises, feel free to leave answer as a definite integral if a closed form solution cannot be found.  
If you can find a closed form solution, you should give that. 
When an arbitrary constant is needed, use $C$.

\begin{exercise}
    Solve $y' + xy = x$.
    
    $y = \answer{1 + Ce^{-x^2}{2}}$
\end{exercise}
%\comboSol{%
%}
%{%
%$y = 1 + Ce^{-x^2}{2}$
%}

\begin{exercise}
    Solve $y' + 6y = e^x$.
    
    $y = \answer{\frac{1}{7}e^x + Ce^{-6x}}$
\end{exercise}
%\comboSol{%
%}
%{%
%$y = \frac{1}{7}e^x + Ce^{-6x}$
%}

\begin{exercise}
    Solve $y' + 4y = x^2e^{-4x}$.
    
    $y = \answer{\frac{1}{3}x^3e^{-4x} + Ce^{-4x}}$
\end{exercise}
%\comboSol{%
%}
%{%
%$y = \frac{1}{3}x^3e^{-4x} + Ce^{-4x}$
%}

\begin{exercise}
    Solve $y' - 3y = xe^x$.
    
    $y = \answer{-\frac{1}{2}xe^{x} - \frac{1}{4}e^x + Ce^{3x}}$
\end{exercise}
%\comboSol{%
%}
%{%
%$y = -\frac{1}{2}xe^{x} - \frac{1}{4}e^x + Ce^{3x}$
%}

\begin{exercise}
    Solve $y' + 3y = e^{4x} - e^{-2x}$ with $y(0) = -3$.
    
    $y = \answer{\frac{1}{7}e^{4x} - e^{-2} + \frac{27}{7}e^{-3x}}$
\end{exercise}
%\comboSol{%
%}
%{%
%$y = \frac{1}{7}e^{4x} - e^{-2} + \frac{27}{7}e^{-3x}$
%}

\begin{exercise}
    Solve $y' - 2y = x + 4$.
    
    $y = \answer{-\frac{x}{2} - \frac{9}{4} + Ce^{2x}}$
\end{exercise}
%\comboSol{%
%}
%{%
%$y = -\frac{x}{2} - \frac{9}{4} + Ce^{2x}$
%}

\begin{exercise}
    Solve $xy' + 4y = x^2 - \frac{1}{x^2}$.
    
    $y = \answer{\frac{x^2}{6} - \frac{1}{2x^2} + Cx^{-4}}$
\end{exercise}
%\comboSol{%
%}
%{%
%$y = \frac{x^2}{6} - \frac{1}{2x^2} + Cx^{-4}$
%}

\begin{exercise}
    Solve $xy' - 3y = x-2$ with $y(1) = 3$. 
    
    $y = \answer{-\frac{1}{2}x - \frac{2}{3} + \frac{25}{6}x^3}$
\end{exercise}
%\comboSol{%
%}
%{%
%$y = -\frac{1}{2}x - \frac{2}{3} + \frac{25}{6}x^3$
%}

\begin{exercise}
    Solve $y' - 4y = \cos{(3t)}$.
    
    $y = \answer{\frac{3}{25}\sin(3t) - \frac{4}{25}\cos(3t) + Ce^{4t}}$
\end{exercise}
%\comboSol{%
%}
%{%
%$y = \frac{3}{25}\sin(3t) - \frac{4}{25}\cos(3t) + Ce^{4t}$
%}

\begin{exercise}%
    Solve $y'+3 x^2 y = x^2$.
    
    $y = \answer{C e^{-x^3} + \frac{1}{3}}$
\end{exercise}
%\exsol{%
%$y = C e^{-x^3} + \frac{1}{3}$
%}

\begin{exercise}
    Solve $y' + 3x^2y = \sin(x) \, e^{-x^3}$, with $y(0) = 1$.
    
    $y = \answer{(2-\cos(x))e^{-x^3}}$
\end{exercise}
%\comboSol{%
%}
%{%
%$y = (2-\cos(x))e^{-x^3}$
%}

\begin{exercise}
    Solve $y' + \cos (x) y = \cos(x)$.
    
    $y = \answer{1 + Ce^{-\sin(x)}}$
\end{exercise}
%\comboSol{%
%}
%{%
%$y = 1 + Ce^{-\sin(x)}$
%}

\begin{exercise}
    Solve the IVP $4ty'+y=24\sqrt{t};\ y(10000)=100.$ %1.4
    
    $y = \answer{8\sqrt{t} - 7000t^{-1/4}}$
\end{exercise}
%\comboSol{%
%}
%{%
%$y = 8\sqrt{t} - 7000t^{-1/4}$
%}

\begin{exercise}
    Solve the IVP $(t^2+1)y' - 2ty = t^2+1; \ y(1)=0$. %1.4
    
    $y = \answer{(t^2 + 1)\left(\tan^{-1}(t) - \frac{\pi}{4}\right)}$
\end{exercise}
%\comboSol{%
%}
%{%
%$y = (t^2 + 1)\left(\tan^{-1}(t) - \frac{\pi}{4}\right)$
%}

\begin{exercise}
    Solve $\frac{1}{x^2+1} \, y' + x y = 3$, with $y(0) = 0$.
    \[
        y = \answer{ e^{-\left(\frac{x^4}{4} + \frac{x^2}{2}\right)}} \int_0^x \answer{3e^{\frac{s^4}{4} + \frac{s^2}{2}}(s^2 + 1) ds}
    \]
\end{exercise}
%\comboSol{%
%}
%{%
%$y = e^{-\left(\frac{x^4}{4} + \frac{x^2}{2}\right)}\int_0^x 3e^{\frac{s^4}{4} + \frac{s^2}{2}}(s^2 + 1)\ ds$
%}

\begin{exercise}%
    Solve $y'+ 2\sin(2x) y = 2\sin(2x)$, $y(\frac{\pi}{2}) = 3$.
    
    $y = \answer{ 2 e^{\cos(2x)+1} + 1}$
\end{exercise}
%\exsol{%
%$y = 2 e^{\cos(2x)+1} + 1$
%}

\begin{exercise}
    Consider the initial value problem
    \[ 
        5y' - 3y = e^{-2t} \qquad y(0) = a 
    \] 
    for an undetermined value $a$. Solve the problem and determine the dependence on the value of $a$. 
    \[
        y = \answer{ -\frac{1}{13}e^{-2t} + \left(a + \frac{1}{13}\right)e^{3/5}t}
    \]
    \begin{problem}
        How does the value of the solution as $t \rightarrow \infty$ depend on the value of $a$?
        \begin{itemize}
            \item If $a > -\frac{1}{13}$, the solution goes to $\answer{\infty}$, 
            \item If $a = -\frac{1}{13}$, the solution goes to $\answer{0}$, 
            \item If $a < -\frac{1}{13}$, the solution goes to $\answer{-\infty}$.
        \end{itemize}
    \end{problem}
\end{exercise}
%\comboSol{%
%}
%{%
%$y = -\frac{1}{13}e^{-2t} + \left(a + \frac{1}{13}\right)e^{3/5}t$. If $a > -\frac{1}{13}$, the solution goes to $\infty$, if $a = -\frac{1}{13}$, the solution goes to 0, if $a < -\frac{1}{13}$, the solution goes to $-\infty$.
%}

\begin{exercise}
    Find an expression for the general solution to $y' + 3y = \sin(t^2)$ with $y(0) = 2$. Simplify your answer as much as possible.
    \[
        y = \answer{ 2e^{-3t} + e^{-3t}}\int_0^t \answer{e^{3s}\sin(s^2) ds}
    \]
\end{exercise}
%\comboSol{%
%}
%{%
%$y = 2e^{-3t} + e^{-3t}\int_0^t e^{3s}\sin(s^2)\ ds$
%}

%\setcounter{exercise}{100}




\end{document}