\documentclass{ximera}

\title{Practice for Substitution}

\input{../../preamble}

\begin{document}
\begin{abstract}
    Why?
\end{abstract}
\maketitle

Hint: Answers need not always be in closed form.

\begin{exercise}
    Solve $y'+ y(x^2-1)+xy^6 = 0$, with $y(1)=1$. 
    \[
        y = \answer{e}^{\answer{x - \frac{x^3}{3}}}\left(\int_{\answer{1}}^{\answer{x}} \answer{5se^{5(s - \frac{s^3}{3})}} ds + \answer{1} \right)^{\answer{-\frac{1}{5}}}
    \]
\end{exercise}
%\comboSol{%
%}
%{%
%$y = e^{x - \frac{x^3}{3}}\left(\int_1^x 5se^{5(s - \frac{s^3}{3})}\ ds + 1 \right)^{-1/5}$
%}

\begin{exercise}%
    Solve $xy'+y+y^2 = 0$, $y(1)=2$. $y = \answer{\frac{2}{3x-2}}$
\end{exercise}
%\exsol{%
%$y = \frac{2}{3x-2}$
%}

\begin{exercise}
    Solve $2yy' + 1 = y^2 + x$, with $y(0)=1$. $y = \answer{(e^x - x)^{\frac{1}{2}}}$
\end{exercise}
%\comboSol{%
%}
%{%
%$y = (e^x - x)^{1/2}$
%}

\begin{exercise}%
    Solve $xy'+y +x = 0$, $y(1)=1$. $y = \answer{\frac{3-x^2}{2 x}}$
\end{exercise}
%\exsol{%
%$y = \frac{3-x^2}{2 x}$
%}

\begin{exercise}
    Solve $y' + xy = y^4$, with $y(0)=1$. $y = \answer{(-3)^{-1/3}e^{-x^2/2}}\left(\int_{\answer{0}}^{\answer{x}} \answer{e^{-3s^2/2}} ds - \answer{\frac{1}{3}} \right)^{\answer{-\frac{1}{3}}}$
\end{exercise}
%\comboSol{%
%}
%{%
%$y = (-3)^{-1/3}e^{-x^2/2}\left(\int_0^x e^{-3s^2/2}\ ds - \frac{1}{3} \right)^{-1/3}$
%}

\begin{exercise}
    Solve $y' + 3y = 2xy^4$. [Use $C$ as your arbitrary constant] $y = \answer{\frac{1}{\left( \frac{2}{3}x + \frac{2}{27} + Ce^{9x}\right)^{\frac{1}{3}}}}$
\end{exercise}
%\comboSol{%
%}
%{%
%$y = \frac{1}{\left( \frac{2}{3}x + \frac{2}{27} + Ce^{9x}\right)^{1/3}}$
%}

\begin{exercise}
    Solve $xy' - 2y = (3x^2 - x^{-3})y^5$ with $y(1) = 2$. $y = \answer{\left(-\frac{6}{5}x^2 + \frac{4}{5}x^{-3} + \frac{1}{80}x^{-8} \right)^{-\frac{1}{4}}}$
\end{exercise}
%\comboSol{%
%}
%{%
%$y = \left( -\frac{6}{5}x^2 + \frac{4}{5}x^{-3} + \frac{!1}{80}x^{-8} \right)^{-1/4}$
%}

\begin{exercise}
    Solve $y' + 5y = \frac{e^{2x}}{y^2}$. [Use $C$ as your arbitrary constant] $y = \answer{\left( \frac{3}{17}e^{2x} + Ce^{-15x} \right)^{\frac{1}{3}}}$
\end{exercise}
%\comboSol{%
%}
%{%
%$y = \left( \frac{3}{17}e^{2x} + Ce^{-15x} \right)^{1/3}$
%}

\begin{exercise}%
    Solve $y^2y' = y^3-3x$, $y(0)=2$. $y = \answer{\bigl(7 e^{3x} + 3x + 1 \bigr)^{\frac{1}{3}}}$
\end{exercise}
%\exsol{%
%$y = {\bigl(7 e^{3x} + 3x + 1 \bigr)}^{1/3}$
%}

\begin{exercise}
    Solve $yy' + x = \sqrt{x^2 + y^2}$. (Hint: What is $\frac{d}{dx}(x^2 + y^2)$) [Use $C$ as your arbitrary constant] $y = \answer{\sqrt{Cx + \frac{x^2}{4}}}$
\end{exercise}
%\comboSol{%
%}
%{%
%$y = \sqrt{Cx + \frac{x^2}{4}}$
%}

\begin{exercise}
    Solve $y' = {(x+y-1)}^2$. [Use $C$ as your arbitrary constant] $y = \answer{\tan(x+C) + 1 - x}$
\end{exercise}
%\comboSol{%
%}
%{%
%$y = \tan(x+C) + 1 - x$
%}

\begin{exercise}
    Solve $y' = \frac{x^2-y^2}{x y}$, with $y(1) = 2$. $y = \answer{\frac{\sqrt{x^4 - 7}}{x\sqrt{2}}}$
\end{exercise}
%\comboSol{%
%}
%{%
%$y = \frac{\sqrt{x^4 - 7}}{x\sqrt{2}}$
%}

\begin{exercise}
    Solve $2yy' = e^{y^2-x^2} + 2x$. [Use $C$ as your arbitrary constant] $y = \answer{\sqrt{x^2-\ln(C-x)}}$
\end{exercise}
%\exsol{%
%$y = \sqrt{x^2-\ln(C-x)}$
%}

\begin{exercise}
    Consider the  DE 
    \begin{equation}
        \frac{dy}{dt}=\left( y -\frac{1}{t} \right)^2 - \frac{1}{t^2}. \label{eq:subsEx1}
    \end{equation} %1.12
    \begin{itemize}
        \item Explain why the DE is not a linear equation.
        \item Use a Bernoulli substitution to solve the DE. [Use $C$ as your arbitrary constant] $y = \answer{\frac{1}{t + Ct^2}}$ 
    \end{itemize}
\end{exercise}
%\comboSol{%
%}
%{%
%a)~ There is a $y^2$ term \quad b)~ $y = \frac{1}{t + Ct^2}$
%}

%\setcounter{exercise}{100}




\end{document}