\documentclass{ximera}

\title{Practice for Non-Homogeneous Equations}

\input{../../preamble}

\begin{document}
\begin{abstract}
    Why?
\end{abstract}
\maketitle

 
\begin{exercise}
    Find a particular solution of $y''-y' -6y = e^{2x}$. [Use $A$ and $B$ as arbitrary constants]
    \[
        y = \answer{Ae^{3x} + Be^{-2x} - \frac{1}{4}e^{2x}}
    \]
\end{exercise}
%\comboSol{%
%}
%{%
%$C_1e^{3x} + C_2e^{-2x} - \frac{1}{4}e^{2x}$
%}

\begin{exercise}
    Find a particular solution of $y''-4y' +4y = e^{2x}$. [Use $A$ and $B$ as arbitrary constants]
    \[
        y = \answer{Ae^{2x} + Bxe^{2x} + \frac{1}{2}x^2e^{2x}}
    \]
\end{exercise}
%\comboSol{%
%}
%{%
%$C_1e^{2x} + C_2xe^{2x} + \frac{1}{2}x^2e^{2x}$
%}

\begin{exercise}%
    Find a particular solution to $y''-y'+y=2\sin(3x)$.
    \[
        y = \answer{\frac{-16\sin(3x)+6\cos(3x)}{73}}
    \]
\end{exercise}
%\exsol{%
%$y=\frac{-16\sin(3x)+6\cos(3x)}{73}$
%}

\begin{exercise}
    Solve the initial value problem $y''+9y = \cos (3x) + \sin (3x)$ for $y(0) = 2$, $y'(0) = 1$.
    \[
        y = \answer{2\cos(3x) + \frac{7}{18}\sin(3x) - \frac{1}{6}x\cos(3x) + \frac{1}{6}x\sin(3x)}
    \]
\end{exercise}
%\comboSol{%
%}
%{%
%$y(x) = 2\cos(3x) + \frac{7}{18}\sin(3x) - \frac{1}{6}x\cos(3x) + \frac{1}{6}x\sin(3x)$
%}

\begin{exercise}
    Set up the form of the particular solution but do not solve for the coefficients for $y^{(4)}-2y'''+y'' = e^x$. [Use $A$ as your arbitrary constant]
    \[
        y = \answer{Ax^2e^x}
    \]
\end{exercise}
%\comboSol{%
%}
%{%
%$Ax^2e^x$
%}

\begin{exercise}
    Set up the form of the particular solution but do not solve for the coefficients for $y^{(4)}-2y'''+y'' = e^x + x + \sin x$. [Use $A$, $B$, $C$, $D$, $E$ as arbitrary constants]
    \[
        y = \answer{Ax^3 + Bx^2 + Cx^2e^x + D\sin(x) + E\cos(x)}
    \]
\end{exercise}
%\comboSol{%
%}
%{%
%$Ax^3 + Bx^2 + Cx^2e^x + D\sin(x) + E\cos(x)$
%}

\begin{exercise}%
    Solve $y''+2y'+y = x^2$, $y(0)=1$, $y'(0)=2$.
    \[
        y = \answer{x^2 - 4x + 6 + e^{-x}(x-5)}
    \]
\end{exercise}
%\exsol{%
%$y(x) = x^2-4 x+6+e^{-x}(x-5)$
%}

\begin{exercise}
    Use the \textit{method of undetermined coefficients} to solve the DE $y''+4y'=2t+30$. [Use $A$ and $B$ as arbitrary constants]
    \[
        y = \answer{A + Be^{-4t} + \frac{1}{4}t + \frac{59}{8}}
    \]
\end{exercise}
%\comboSol{%
%}
%{%
%$y(t) = C_1 + C_2e^{-4t} + \frac{1}{4}t + \frac{59}{8}$
%}

\begin{exercise}
    Using variation of parameters find a particular solution of $y''-2y'+y = e^x$.
    \[
        y = \answer{\frac{x^2}{2}e^x}
    \]
%    
%        \task Find a particular solution using undetermined coefficients.
%        \task Are the two solutions you found the same? See also \exerciseref{exercise:diffvarparunder}.
%    \end{tasks}
\end{exercise}
%\comboSol{%
%}
%{%
%$\frac{x^2}{2}e^x$
%}


\begin{exercise}%
    Find a particular solution to $y''+2y=e^x + x^3$. $y=\answer{\frac{2e^x+3x^3-9x}{6}}$
    
    \begin{problem}
        Find the general solution. [Use $A$ and $B$ as arbitrary constants]
        \[
            y=\answer{A \cos(\sqrt{2} x) + B \sin(\sqrt{2} x) + \frac{2e^x+3x^3-9x}{6}}
        \]
    \end{problem}
\end{exercise}

%\exsol{%
%a) $y=\frac{2e^x+3x^3-9x}{6}$ \quad
%b) $y=C_1 \cos(\sqrt{2} x) + C_2 \sin(\sqrt{2} x) + \frac{2e^x+3x^3-9x}{6}$
%}

\begin{exercise}
    Find the general solution to $y'' - 3y' - 4y = e^{2t} + 1$. [Use $A$ and $B$ as arbitrary constants]
    \[
        y=\answer{A e^{4t} + B e^{-t} - \frac{1}{6}e^{2t} - \frac{1}{4}}
    \]
\end{exercise}
%\comboSol{%
%}
%{%
%$y(t) = C_1e^{4t} + C_2e^{-t} - \frac{1}{6}e^{2t} - \frac{1}{4}$
%}

\begin{exercise}
    Find the general solution to $y'' - 2y' + 5y = \sin(3t) + 2\cos(3t)$. [Use $A$ and $B$ as arbitrary constants]
    \[
        y=\answer{A e^t\cos(2t) + Be^t\sin(2t) - \frac{4}{13}\sin(3t) - \frac{1}{26}\cos(3t)}
    \]
\end{exercise}
%\comboSol{%
%}
%{%
%$y(t) = C_1e^t\cos(2t) + C_2e^t\sin(2t) - \frac{4}{13}\sin(3t) - \frac{1}{26}\cos(3t)$
%}

\begin{exercise}
    Find the general solution to $y'' - 4y' - 21y = e^{-3t} + e^{4t}$. [Use $A$ and $B$ as arbitrary constants]
    \[
        y=\answer{A e^{7t} + Be^{-3t} - \frac{1}{10}te^{-3t} - \frac{1}{21}e^{4t}}
    \]
\end{exercise}
%\comboSol{%
%}
%{%
%$y(t) = C_1e^{7t} + C_2e^{-3t} - \frac{1}{10}te^{-3t} - \frac{1}{21}e^{4t}$
%}

\begin{exercise}
    Find the general solution to $y'' - 2y' + y = e^t - t$. [Use $A$ and $B$ as arbitrary constants]
    \[
        y=\answer{A e^t + Bte^t + \frac{1}{2}t^2e^t - t - 2}
    \]
\end{exercise}
%\comboSol{%
%}
%{%
%$y(t) = C_1e^t + C_2te^t + \frac{1}{2}t^2e^t - t - 2$
%}

\begin{exercise}
    Find the general solution to $y'' + 4y = \sec(2t)$ using variation of parameters. [Use $A$ and $B$ as arbitrary constants]
    \[
        y=\answer{A \cos(2t) + B\sin(2t) + \frac{1}{4}\cos(2t)\ln(\cos(2t)) + \frac{1}{2}t\sin(2t)}
    \]
\end{exercise}
%\comboSol{%
%}
%{%
%$y(t) = C_1\cos(2t) + C_2\sin(2t) + \frac{1}{4}\cos(2t)\ln(\cos(2t)) + \frac{1}{2}t\sin(2t)$
%}

\begin{exercise}
    Find the solution of the initial value problem $y'' - 2y' - 15y = e^{5t} + 3$, $y(0) = 2$, $y'(0) = -1$.
    \[
        y=\answer{\frac{219}{320}e^{5t} + \frac{97}{64}e^{-3t} + \frac{1}{8}te^{5t} - \frac{1}{5}}
    \]
\end{exercise}
%\comboSol{%
%}
%{%
%$y(t) = \frac{219}{320}e^{5t} + \frac{97}{64}e^{-3t} + \frac{1}{8}te^{5t} - \frac{1}{5}$
%}

\begin{exercise}
    Find the solution of the initial value problem $y'' + 4y' + 5y = \cos(3t) + t$, $y(0) = 0$, $y'(0) = 2$.
        \[
            y=\answer{\frac{37}{200}e^{-2t}\cos(t) + \frac{389}{200}e^{-2t}\sin(t) - \frac{1}{40}\cos(3t) + \frac{3}{40}\sin(3t) + \frac{t}{5} - \frac{4}{25}}
        \]
\end{exercise}
%\comboSol{%
%}
%{%
%$y(t) = \frac{37}{200}e^{-2t}\cos(t) + \frac{389}{200}e^{-2t}\sin(t) - \frac{1}{40}\cos(3t) + \frac{3}{40}\sin(3t) + \frac{t}{5} - \frac{4}{25}$
%}

\begin{exercise}
    The following differential equations are all related. Find the general solution to each of them. [Use $A$ and $B$ for arbitrary coefficients]% and compare and contrast the different solutions and the methods used to approach them.
    \begin{itemize}
        \item $y'' - 2y' - 15y = e^t + 5e^{-4t}$
        \[
            y = \answer{Ae^{5t} + Be^{-3t}  - \frac{1}{16}e^t + \frac{5}{9}e^{-4t}}
        \]
        \item $y'' - 2y' - 15y = 2e^{2t} + 3e^{-t}$
        \[
            y = \answer{Ae^{5t} + Be^{-3t}  - \frac{2}{15}e^{2t} - \frac{3}{13}e^{-t}}
        \]
        \item $y'' - 2y' - 15y = 3\cos(2t)$
        \[
            y = \answer{Ae^{5t} + Be^{-3t}  - \frac{57}{377}\cos(2t) - \frac{12}{377}\sin(2t)}
        \]
        \item $y'' - 2y' - 15y = 2e^{5t} - \sin(t)$
        \[
            y = \answer{Ae^{5t} + Be^{-3t}  + \frac{1}{4}te^{5t} - \frac{1}{130}\cos(t) + \frac{4}{65}\sin(t)}
        \]
    \end{itemize}
\end{exercise}
%\comboSol{%
%}
%{%
%a)~$C_1e^{5t} + C_2e^{-3t}  - \frac{1}{16}e^t + \frac{5}{9}e^{-4t}$ \quad b)~$C_1e^{5t} + C_2e^{-3t}  - \frac{2}{15}e^{2t} - \frac{3}{13}e^{-t}$ \\
%c)~$C_1e^{5t} + C_2e^{-3t}  - \frac{57}{377}\cos(2t) - \frac{12}{377}\sin(2t)$ \quad d)~$C_1e^{5t} + C_2e^{-3t}  + \frac{1}{4}te^{5t} - \frac{1}{130}\cos(t) + \frac{4}{65}\sin(t)$ \\
%}

\begin{exercise}
    The following differential equations are all related. Find the general solution to each of them. [Use $A$ and $B$ for arbitrary coefficients]% and compare and contrast the different solutions and the methods used to approach them.
    \begin{itemize}
        \item $y'' + 4y' + 3y = e^{2t} + 3e^{4t}$ 
        \[
            y = \answer{Ae^{-t} + Be^{-3t} + \frac{1}{11}e^{2t} + \frac{3}{35}e^{4t}}
        \]
        \item $y'' - 2y' + 5y = e^{2t} + 3e^{4t}$
        \[
            y = \answer{AC_1e^{t}\cos(2t) + Be^t\sin(2t) + \frac{1}{20}e^{2t} + \frac{3}{13}e^{4t}}
        \]
        \item $y'' + 3y' - 10y = e^{2t} + 3e^{4t}$
        \[
            y = \answer{Ae^{-5t} + Be^{2t} + \frac{1}{7}te^{2t} - \frac{1}{2}e^{4t}}
        \]
        \item $y'' - 8y'  + 16y = e^{2t} + 3e^{4t}$
        \[
            y = \answer{Ae^{4t} + Bte^{4t} - \frac{1}{28}e^{2t} + \frac{3}{2}t^2e^{4t}}
        \]
    \end{itemize}
\end{exercise}
%\comboSol{%
%}
%{%
%a)~$C_1e^{-t} + C_2e^{-3t} + \frac{1}{11}e^{2t} + \frac{3}{35}e^{4t}$ \quad b)~$C_1e^{t}\cos(2t) + C_2e^t\sin(2t) + \frac{1}{20}e^{2t} + \frac{3}{13}e^{4t}$ \\ c)~$C_1e^{-5t} + C_2e^{2t} + \frac{1}{7}te^{2t} - \frac{1}{2}e^{4t}$ \quad d)~$C_1e^{4t} + C_2te^{4t} - \frac{1}{28}e^{2t} + \frac{3}{2}t^2e^{4t}$
%}

\begin{exercise}
    Find a particular solution of $y''-2y' +y = \sin (x^2)$.  It is OK to leave the answer as a definite integral.
    \[
        y = \answer{e^x}\int_0^x \answer{se^{-s}\sin(s^2)} ds + x\answer{e^x}\int_0^x \answer{e^{-s}\sin(s^2)} ds
    \]
\end{exercise}
%\comboSol{%
%}
%{%
%$e^x\int_0^x se^{-s}\sin(s^2)\ ds + xe^x\int_0^xe^{-s}\sin(s^2)\ ds$
%}

\begin{exercise}
    Use variation of parameters to find a particular solution of $y''-y = \frac{1}{e^x+e^{-x}}$.
    \[
        y = \answer{\frac{2xe^x-(e^x+e^{-x})\log(e^{2x}+1)}{4}}
    \]
\end{exercise}
%\exsol{%
%$y = \frac{2xe^x-(e^x+e^{-x})\log(e^{2x}+1)}{4}$
%}

\begin{exercise}
    Recall that a homogeneous Euler equation is one of the form $t^2y'' + aty' + by = 0$ and is solved by using the guess $y(t) = t^r$ and solving for the potential values of $r$. 
    \begin{itemize}
        \item Solve $t^2y''-2ty'-10y=0$. [Use $A$ and $B$ as your arbitrary constants]%2.5, Euler eq
        \[
            y(t) = \answer{At^5 + Bt^{-2}}
        \]
        \item Let $y_1$ and $y_2$ be a fundamental set for the above equation. Use the variation of parameters equations $u_1=-\int \frac{y_2 g(t)}{y_1y_2' - y_2y_1'}dt$, $y_2=\int \frac{y_1 g(t)}{y_1y_2' - y_2y_1'}dt$ to solve the non-homogeneous equation $y''-\frac{2}{t} - \frac{10}{t^2}=t^3$. (Do not attempt method of undetermined coefficients instead; it won't work.)
        \[
            y(t) = \answer{At^5 + Bt^{-2} + t^5\left(\frac{1}{7}\ln(|t|) - \frac{1}{49}\right)}
        \]
    \end{itemize}
\end{exercise}
%\comboSol{%
%}
%{%
%a)~$y(t) = C_1t^5 + C_2t^{-2}$ \quad
%b)~$y(t) = C_1t^5 + C_2t^{-2} + t^5\left(\frac{1}{7}\ln(|t|) - \frac{1}{49}\right)$
%}

\begin{exercise}
    For an arbitrary constant $c$ find the general solution to $y''-2y=\sin(x+c)$. [Use $A$ and $B$ as your arbitrary constants beyond the given $c$]
    \[
        y=\answer{\frac{-\sin(x+c)}{3} + A e^{\sqrt{2}x} + B e^{-\sqrt{2}x}}
    \]
\end{exercise}
%\exsol{%
%$y=\frac{-\sin(x+c)}{3}+C_1 e^{\sqrt{2}x}+C_2 e^{-\sqrt{2}x}$
%}

\begin{exercise}
    For an arbitrary constant $c$ find a particular solution to $y''-y=e^{cx}$.  Hint: Make sure to handle every possible real $c$. [Use $A$ and $B$ as your arbitrary constants beyond the given $c$]
    \begin{itemize}
        \item For $c\neq \pm \answer{1}$: $y=\answer{Ae^x + Be^{-x} + \frac{1}{c^2 - 1}e^{cx}}$
        \item For $c = + \answer{1}$: $y=\answer{Ae^x + Be^{-x} + \frac{1}{2}xe^x}$
        \item For $c = - \answer{1}$: $y=\answer{Ae^x + Be^{-x} - \frac{1}{2}xe^{-x}}$
    \end{itemize}
\end{exercise}
%\comboSol{%
%}
%{%
%$c\neq \pm1$: $C_1e^x + C_2e^{-x} + \frac{1}{c^2 - 1}e^{cx}$, \ $c=1$: $C_1e^x + C_2e^{-x} + \frac{1}{2}xe^x$, \ $c=-1$: $C_1e^x + C_2e^{-x} - \frac{1}{2}xe^{-x}$
%}

\begin{exercise} \label{exercise:diffvarparunder}
    \begin{itemize}
        \item Using variation of parameters find a particular solution of $y''-y = e^x$.
        \[
            y = \answer{\frac{1}{2}xe^x - \frac{1}{4}e^x}
        \]
        \item Find a particular solution using undetermined coefficients.
        \[
            y = \answer{\frac{1}{2}xe^x}
        \]
        \item Are the two solutions you found the same? What is going on? [Use C for arbitrary constant]
        \[
            \text{They differ by: } \answer{Ce^x}
        \]
    \end{itemize}
\end{exercise}
%\comboSol{%
%}
%{%
%a)~$\frac{1}{2}xe^x - \frac{1}{4}e^x$ \quad b)~$\frac{1}{2}xe^x$ \quad c)~They differ by a $Ce^x$ term
%}

%\setcounter{exercise}{100}



\end{document}