\documentclass{ximera}

\title{Practice for Second Order Repeated Roots}

\input{../../preamble}

\begin{document}
\begin{abstract}
    Why?
\end{abstract}
\maketitle



\begin{exercise}
    Find the general solution to $y'' + 4y' + 4y = 0$. Use $A$ and $B$ for your arbitrary constants. $y = \answer{Ae^{-2t} + Bte^{-2t}}$
\end{exercise}
%\comboSol{%
%}
%{%
%$C_1e^{-2t} + C_2te^{-2t}$
%}

\begin{exercise}%
    Find the general solution to $y''-6y'+9y=0$. Use $A$ and $B$ for your arbitrary constants. $y = \answer{Ae^{3x} + Bx e^{3x}}$
\end{exercise}
%\exsol{%
%$y =
%C_1 e^{3x} + C_2 x e^{3x}$
%}


\begin{exercise}
    Find the solution to $y'' + 6y' + 9y = 0$ with $y(0) = 3$ and $y'(0) = -1$. $y = \answer{3e^{-3t} + 8te^{-3t}}$
\end{exercise}
%\comboSol{%
%}
%{%
%$y = 3e^{-3t} + 8te^{-3t}$
%}

\begin{exercise}
    Solve $y'' - 8y' + 16 y = 0$ for $y(0) = 2$, $y'(0) = 0$. $y = \answer{2e^{4t} - 8te^{4t}}$
\end{exercise}
%\comboSol{%
%}
%{%
%$y = 2e^{4t} - 8te^{4t}$
%}

\begin{exercise}
    Find the general solution of $y'' = 0$ using the methods of this section. Use $A$ and $B$ for your arbitrary constants. $y = \answer{A + Bt}$
\end{exercise}
%\comboSol{%
%}
%{%
%$C_1 + C_2t$
%}

\begin{exercise}
    The method of this section applies to equations of other orders than two. We will see higher orders later.  Try to solve the first order equation $2y' + 3y = 0$ using the methods of this section. Use $A$ for your arbitrary constant. $y = \answer{Ae^{-\frac{3t}{2}}}$
\end{exercise}
%\comboSol{%
%}
%{%
%$Ce^{-3t/2}$
%}

\begin{exercise}
    Consider the second-order DE 
    \begin{equation}
        ty''+(4t+2)y'+(4t+4)y=0. \label{eq:2_3_Exercise1}
    \end{equation}
    Does the \textit{superposition principle} apply to this DE? %Give a one- or two-sentence explanation wither way.
    \begin{multipleChoice}
        \choice[correct]{Yes.}
        \choice{No.}
    \end{multipleChoice}
    \begin{feedback}[correct]
        Try coming up with a one or two sentence explanation of why.
    \end{feedback}
    \begin{problem}
        Find a value of $r$ so that $y=e^{rt}$ is a solution to the given DE. $r = \answer{-2}$
        \begin{problem}
            Using the previous result, apply \textbf{reduction of order} to find the general solution to the original DE. [Use $A$ and $B$ as your arbitrary constants]
            \[
                y = \answer{Ae^{-2t} + B\frac{e^{-2t}}{t}}
            \]
        \end{problem}
    \end{problem}
\end{exercise}
%\comboSol{%
%}
%{%
%a)~Yes, it is linear \quad b)~ $r=-2$ \quad c)~ $y = C_1e^{-2t} + C_2\frac{e^{-2t}}{t}$
%}

\begin{exercise}%[Euler Equations]%
    Consider the differential equation $x^2y'' + 3xy' - 3y = 0$.
    Start by verifying that $y_1(x) = x$ is a solution.
    Then use reduction of order to find a second linearly independent solution.
    
    Finally, write out the general solution. [Use $A$ and $B$ as your arbitrary constants] 
    \[
        y(x) = \answer{Ax + B\frac{1}{x^3}}
    \]
\end{exercise}
%\exsol{%
%c) $y(x) = C_1 x + C_2\frac{1}{x^3}$
%}

\begin{exercise}%[Euler Equations]%
    Consider the differential equation $x^2y'' + 4xy' + 2y = 0$.
    Start by verifying that $y_1(x) = \frac{1}{x}$ is a solution.
    Then use reduction of order to find a second linearly independent solution.
    
    Finally write out the general solution. [Use $A$ and $B$ as your arbitrary constants]
    \[
        y(x) = \answer{A \frac{1}{x} + B x^4}
    \]
\end{exercise}
%\exsol{%
%c) $y(x) = C_1 \frac{1}{x} + C_2 x^4$
%}

\begin{exercise}%[Euler Equations]%
    Consider the differential equation $x^2y'' -6xy' + 10y = 0$.
    Start by verify that $y_1(x) = x^2$ is a solution.
    Then use reduction of order to find a second linearly independent solution.
    
    Finally write out the general solution. [Use $A$ and $B$ as your arbitrary constants] 
    \[
        y(x) = \answer{A x^2 + B x^{5}}
    \]

\end{exercise}
%\exsol{%
%c) $y(x) = C_1 x^2 + C_2 x^{5}$
%}

\begin{exercise}
    Write down a differential equation with general solution $y=at^2+bt^{-3}$. [Use $\frac{d^2y}{dx^2}$ for $y''$ and $\frac{dy}{dx}$ for $y'$. Make sure to enter the full equality.]
    \[
        \answer{x^2\frac{d^2y}{dx^2} + 2x\frac{dy}{dx} - 6y = 0}
    \]
\end{exercise}
%\comboSol{%
%}
%{%
%$x^2y'' + 2xy' - 6y = 0$
%}

\begin{exercise}
    Find the solution to $y''-(2\alpha) y' + \alpha^2 y=0$, $y(0) = a$, $y'(0)=b$, where $\alpha$, $a$, and $b$ are real numbers.
    \[
        y = \answer{ae^{\alpha t} + (b - \alpha a)te^{\alpha t}}
    \]
\end{exercise}
%\comboSol{%
%}
%{%
%$y = ae^{\alpha t} + (b - \alpha a)te^{\alpha t}$
%}

\begin{exercise}[reduction of order] \label{exercise:reductionoforder}
    Suppose $y_1$ is a solution to $y'' + p(x) y' + q(x) y = 0$. By directly plugging into the equation, show that
    \begin{equation*}
        y_2(x) = y_1(x) \int \frac{e^{-\int p(x)\,dx}}{{\bigl(y_1(x)\bigr)}^2} \,dx
    \end{equation*}
    is also a solution.
\end{exercise}
%\comboSol{%
%}
%{%
%Yes
%}

\begin{exercise}%[\myindex{Chebyshev's equation of order 1}]
    Take $(1-x^2)y''-xy' + y = 0$.
    \begin{tasks}
        \task Show that $y=x$ is a solution.
        \task Use reduction of order to find a second linearly independent solution.
        \task Write down the general solution.
    \end{tasks}
\end{exercise}
%\comboSol{%
%}
%{%
%a)~Works \quad b)~$y_2(x) = \sqrt{1 - x^2}$ \quad c)~ $C_1x + C_2\sqrt{1-x^2}$
%}

\begin{exercise}%[\myindex{Hermite's equation of order 2}]
    Take $y''-2xy' + 4y = 0$.
    First show that $y=1-2x^2$ is a solution.  
    \begin{problem}
        Use reduction of order to find a second linearly independent solution. (It's OK to leave a definite integral in the formula.)
        \[
            y_2(x) = \left(\answer{1-2x^2}\right)\int\limits_{\answer{0}}^{\answer{x}} \answer{e^{s^2}(2s^2 - 1)^{-2}}ds
        \]
        \begin{problem}
            Write down the general solution. [Use $A$ and $B$ as arbitrary constants]
            \[
                \answer{A(1-2x^2) + B(1-2x^2)}\int_0^x\answer{e^{s^2}(2s^2 - 1)^{-2}} ds
            \]
        \end{problem}
    \end{problem}
\end{exercise}
%\comboSol{%
%}
%{%
%a)~ Works \quad b)~$y_2(x) = (1-2x^2)\int_0^xe^{s^2}(2s^2 - 1)^{-2}\ ds$ \\ c)~ $C_1(1-2x^2) + C_2(1-2x^2)\int_0^xe^{s^2}(2s^2 - 1)^{-2}\ ds$
%}

\noindent The rest of these exercises can be solved using any of the methods discussed in the last three sections. Pick the appropriate method in order to solve the problem.

\begin{exercise}
    Find the general solution of $y'' + 5y' - 6y = 0$. [Use $A$ and $B$ as arbitrary constants]
    \[
        y = \answer{Ae^{-6t} + Be^t}
    \]
\end{exercise}
%\comboSol{%
%}
%{%
%$C_1e^{-6t} + C_2e^t$
%}

\begin{exercise}
    Find the general solution of $y'' - 2y' + 2y = 0$. [Use $A$ and $B$ as arbitrary constants]
    \[
        y = \answer{Ae^t\cos(t) + Be^t\sin(t)}
    \]
\end{exercise}
%\comboSol{%
%}
%{%
%$C_1e^t\cos(t) + C_2e^t\sin(t)$
%}

\begin{exercise}
    Find the general solution of $y'' + 4y' + 4y = 0$. [Use $A$ and $B$ as arbitrary constants]
    \[
        y = \answer{Ae^{-2t} + Bte^{-2t}}
    \]
\end{exercise}
%\comboSol{%
%}
%{%
%$C_1e^{-2t} + C_2te^{-2t}$
%}

\begin{exercise}
    Find the general solution of $y'' + 4y' + 5y = 0$. [Use $A$ and $B$ as arbitrary constants]
    \[
        y = \answer{Ae^{-2t}\cos(t) + Be^{-2t}\sin(t)}
    \]
\end{exercise}
%\comboSol{%
%}
%{%
%$C_1e^{-2t}\cos(t) + C_2e^{-2t}\sin(t)$
%}

\begin{exercise}
    Find the solution to $y'' - 6y' + 13y = 0$ with $y(0) = 2$ and $y'(0) = 1$. 
    \[
        y = \answer{2e^{3t}\cos(2t) - \frac{5}{2}e^{3t}\sin(2t)}
    \]
\end{exercise}
%\comboSol{%
%}
%{%
%$y = 2e^{3t}\cos(2t) - \frac{5}{2}e^{3t}\sin(2t)$
%}

\begin{exercise}
    Find the solution to $y'' + 4y' - 12y = 0$ with $y(0) = -1$ and $y'(0) = 3$. 
    \[
        y = \answer{-\frac{4}{5}e^{-6t} - \frac{1}{5}e^{2t}}
    \]
\end{exercise}
%\comboSol{%
%}
%{%
%$y= -\frac{4}{5}e^{-6t} - \frac{1}{5}e^{2t}$
%}

\begin{exercise}
    Find the solution to $y'' - 6y' + 9y = 0$ with $y(0) = -4$ and $y'(0) = -1$. 
    \[
        y = \answer{-3e^{3t} + 11te^{3t}}
    \]
\end{exercise}
%\comboSol{%
%}
%{%
%$y = -3e^{3t} + 11te^{3t}$
%}

\end{document}